src/program_proof/simplepb/apps/closed_wpcs.v
@@ -1,0 +1,83 @@
+From Perennial.program_proof Require Import grove_prelude.
+From Goose.github_com.mit_pdos.gokv.simplepb.apps Require Import closed.
+
+From Perennial.goose_lang Require adequacy dist_adequacy.
+From Perennial.goose_lang.ffi Require grove_ffi_adequacy.
+From Perennial.program_logic Require dist_lang.
+
+From Perennial.program_proof.simplepb Require Import config_proof pb_definitions pb_ghost pb_init_proof.
+From Perennial.program_proof.simplepb Require Import kv_proof.
+From Perennial.program_proof.simplepb.simplelog Require Import proof.
+From Perennial.program_proof.grove_shared Require Import urpc_proof.
+From Perennial.goose_lang Require Import crash_borrow crash_modality.
+
+Section closed_wpcs.
+
+(* FIXME: kv64G *)
+Context `{!heapGS Σ}.
+Context `{!urpc_proof.urpcregG Σ}.
+Context `{!simplelogG (sm_record:=kv_record) Σ}.
+Context `{!ghost_mapG Σ u64 (list u8)}.
+
+Definition replica_fname := "kv.data".
+
+Lemma wpc_kv_replica_main1 γsys γsrv :
+  is_pb_host 1%Z γsys γsrv -∗ sys_inv γsys -∗
+  (∃ data : list u8, replica_fname f↦data ∗ file_crash (own_Server_ghost γsys γsrv) data) -∗
+  WPC kv_replica_main1 #() @ ⊤
+  {{ _, True }}
+  {{ ∃ data' : list u8, replica_fname f↦data' ∗ ▷ file_crash (own_Server_ghost γsys γsrv) data' }}
+.
+Proof.
+  iIntros "#Hpbhots #Hsys Hpre".
+  iDestruct "Hpre" as (?) "[Hfile Hcrash]".
+
+  unfold kv_replica_main1.
+  wpc_call.
+  { iExists _. iFrame. }
+
+  iCache with "Hfile Hcrash".
+  { iExists _. iFrame. }
+  wpc_bind (Primitive2 _ _ _).
+  wpc_frame.
+  iApply wp_crash_borrow_generate_pre.
+  { done. }
+  wp_apply (wp_ref_of_zero).
+  { done. }
+  iIntros (?) "Hl".
+  iIntros "Hpreborrow".
+  iNamed 1.
+  wpc_pures.
+  wpc_bind (store_ty _ _).
+  wpc_frame.
+  wp_store.
+  iModIntro.
+  iNamed 1.
+
+  iApply wpc_cfupd.
+  wpc_apply (wpc_crash_borrow_inits with "Hpreborrow [Hfile Hcrash] []").
+  { iAccu. }
+  {
+    iModIntro.
+    instantiate (1:=(|C={⊤}=> ∃ data', replica_fname f↦ data' ∗ ▷ file_crash (own_Server_ghost γsys γsrv) data')).
+    iIntros "[H1 H2]".
+    iModIntro.
+    iExists _.
+    iFrame.
+  }
+  iIntros "Hfile_ctx".
+  wpc_apply (wpc_crash_mono _ _ _ _ _ (True%I) with "[]").
+  { iIntros "_".
+    iIntros "$". }
+  iApply wp_wpc.
+  wp_pures.
+
+  wp_apply (wp_Start with "[Hfile_ctx]").
+  {
+    iFrame "∗#".
+  }
+  wp_pures.
+  done.
+Qed.
+
+End closed_wpcs.
